

### Problem #6

$$\begin{aligned} 1. m(a+bX) &= \frac{1}{N} \sum_{i=1}^N (a + bX_i) \\ &= \frac{1}{N} \left( \sum_{i=1}^N a + b \sum_{i=1}^N X_i \right) \\ &= a + b \left( \frac{1}{N} \sum_{i=1}^N X_i \right) \end{aligned}$$

$$\therefore m(a+bX) = a + b \cdot m(X)$$

$$\begin{aligned} 2. \text{cov}(X, X) &= \frac{1}{N} \sum_{i=1}^N (X_i - m(X)) (X_i - m(X)) \\ &= \frac{1}{N} \sum_{i=1}^N (X_i - m(X))^2 \\ \text{cov}(X, X) &= s^2 \end{aligned}$$

$$\begin{aligned} 3. \text{cov}(X, a+bY) &= \frac{1}{N} \sum_{i=1}^N (X_i - m(X)) [(a+bY_i) - (a+bm(Y))] \\ &= \frac{1}{N} \sum_{i=1}^N (X_i - m(X)) (a+bY_i - a - bm(Y)) \\ &= \frac{1}{N} \sum_{i=1}^N (X_i - m(X)) [b(Y_i - m(Y))] \end{aligned}$$

$$\text{cov}(X, a+bY) = b \text{cov}(X, Y)$$

$$\begin{aligned} 4. \text{cov}(a+bX, a+bY) &= \frac{1}{N} \sum_{i=1}^N [(a+bX_i) - (a+bm(X))] [(a+bY_i) - (a+bm(Y))] \\ &= \frac{1}{N} \sum_{i=1}^N (a+bX_i - a - bm(X)) (a+bY_i - a - bm(Y)) \\ &= \frac{1}{N} \sum_{i=1}^N b(X_i - m(X)) \cdot b(Y_i - m(Y)) \\ &= \frac{1}{N} \sum_{i=1}^N b^2 (X_i - m(X)) (Y_i - m(Y)) \end{aligned}$$

$$\text{cov}(a+bX, a+bY) = b^2 \text{cov}(X, Y)$$

5.  $b > 0$ , median of  $X = \text{med}(X)$

$$\text{Yes, } a+bX = a+b \cdot \text{med}(X)$$

$$\text{IQR} = Q_2 - Q_1$$

↳ order is preserved

$$\text{IQR}(a+bX) = (a+bQ_2) - (a+bQ_1)$$

$$= a+bQ_2 - a-bQ_1$$

6. ex.:  $X = \{3, 5\}$

$$m(X) = 4$$

$$m(X^2) = \frac{9+25}{2} = \frac{34}{2} = 17$$

$$(m(X))^2 = 4^2 = 16$$

$$\begin{aligned} \text{IQR}(a+bX) &\neq b(\text{IQR}(X)) = b(Q_2 - Q_1) \\ &= b(\text{IQR}(X)) \end{aligned}$$

$$\left\{ \begin{aligned} (m(X))^2 &\neq m(X^2) \end{aligned} \right.$$

$$m(\sqrt{X}) = \frac{\sqrt{3} + \sqrt{5}}{2} = \frac{3.968}{2} = 1.984$$

$$\sqrt{m(X)} = \sqrt{4} = 2$$

$$\left\{ \begin{aligned} m(\sqrt{X}) &\neq \sqrt{m(X)} \end{aligned} \right.$$